V4

docs/paper/demo.v
@@ -122,20 +122,19 @@ Elpi hb.declare_factory Ring_of_Monoid A Monoid.axioms.
 
   Variable f : axioms.
 
-Lemma addrC : commutative (add : A -> A -> A).
-Proof.
-have addKl (a b c : A) : a + b = a + c -> b = c.
-  apply: can_inj (add a) (add (opp f a)) _ _ _.
-  by move=> x; rewrite addrA (addNr f) add0r.
-have addKr (a b c : A) : b + a = c + a -> b = c.
-  apply: can_inj (add ^~ a) (add ^~ (opp f a)) _ _ _.
-  by move=> x; rewrite /= -addrA (addrN f) addr0.
-have innerC (a b : A) : a + b + (a + b) = a + a + (b + b).
-  by rewrite -[a+b](mul1r f) -(mulrDl f) (mulrDr f) !(mulrDl f) !(mul1r f).
-move=> x y; apply: addKl (x) _ _ _; apply: addKr (y) _ _ _.
-by rewrite -!addrA [in RHS]addrA innerC !addrA.
-Qed.
-
+  Lemma addrC : commutative (add : A -> A -> A).
+  Proof.
+  have addKl (a b c : A) : a + b = a + c -> b = c.
+    apply: can_inj (add a) (add (opp f a)) _ _ _.
+    by move=> x; rewrite addrA (addNr f) add0r.
+  have addKr (a b c : A) : b + a = c + a -> b = c.
+    apply: can_inj (add ^~ a) (add ^~ (opp f a)) _ _ _.
+    by move=> x; rewrite /= -addrA (addrN f) addr0.
+  have innerC (a b : A) : a + b + (a + b) = a + a + (b + b).
+    by rewrite -[a+b](mul1r f) -(mulrDl f) (mulrDr f) !(mulrDl f) !(mul1r f).
+  move=> x y; apply: addKl (x) _ _ _; apply: addKr (y) _ _ _.
+  by rewrite -!addrA [in RHS]addrA innerC !addrA.
+  Qed.
 
   Definition to_AbelianGroup_of_Monoid :=
     AbelianGroup_of_Monoid.Axioms A (opp f) addrC (addNr f).
@@ -149,6 +148,134 @@ Qed.
 Elpi hb.end.
 
 End V3.
+
+Module V4.
+
+Elpi hb.declare_mixin Monoid_of_Type A.
+  Record axioms := {
+    zero : A;
+    add : A -> A -> A;
+    addrA : associative add;
+    add0r : left_id zero add;
+    addr0 : right_id zero add;
+  }.
+Elpi hb.end.
+Elpi hb.structure Monoid Monoid_of_Type.axioms.
+
+Elpi hb.declare_mixin AbelianGroup_of_Monoid A Monoid.axioms.
+  Record axioms := {
+    opp : A -> A;
+    addrC : commutative (add : A -> A -> A);
+    addNr : left_inverse zero opp add;
+  }.
+Elpi hb.end.
+Elpi hb.structure AbelianGroup Monoid.axioms AbelianGroup_of_Monoid.axioms.
+
+Elpi hb.declare_mixin SemiRing_of_Monoid A Monoid.axioms.
+  Record axioms := {
+    one : A;
+    mul : A -> A -> A;
+    mulrA : associative mul;
+    mul1r : left_id one mul;
+    mulr1 : right_id one mul;
+    mulrDl : left_distributive mul add;
+    mulrDr : right_distributive mul add;
+    mul0r : left_zero zero mul;
+    mulr0 : right_zero zero mul;
+  }.
+Elpi hb.end.
+Elpi hb.structure SemiRing Monoid.axioms SemiRing_of_Monoid.axioms.
+
+Declare Scope hb_scope.
+Delimit Scope hb_scope with G.
+Open Scope hb_scope.
+Notation "0" := zero : hb_scope.
+Notation "1" := one : hb_scope.
+Infix "+" := (@add _) : hb_scope.
+Notation "- x" := (@opp _ x) : hb_scope.
+Infix "*" := (@mul _) : hb_scope.
+Notation "x - y" := (x + - y) : hb_scope.
+
+Lemma addrN {R : AbelianGroup.type} : right_inverse (zero : R) opp add.
+Proof. by move=>x; rewrite addrC addNr. Qed.
+
+Elpi hb.declare_factory Ring_of_AbelianGroup A AbelianGroup.axioms.
+  Record axioms := {
+    one : A;
+    mul : A -> A -> A;
+    mulrA : associative mul;
+    mul1r : left_id one mul;
+    mulr1 : right_id one mul;
+    mulrDl : left_distributive mul add;
+    mulrDr : right_distributive mul add;
+  }.
+
+  Variable f : axioms.
+
+  Fact mul0r : left_zero zero (mul f).
+  Proof.
+  move=> x; rewrite -[LHS]add0r addrC.
+  rewrite -{2}(addNr (mul f x x)) (addrC (opp _)) addrA.
+  by rewrite -mulrDl add0r addrC addNr.
+  Qed.
+
+  Fact mulr0 : right_zero zero (mul f).
+  Proof.
+  move=> x; rewrite -[LHS]add0r addrC.
+  rewrite -{2}(addNr (mul f x x)) (addrC (opp _)) addrA.
+  by rewrite -mulrDr add0r addrC addNr.
+  Qed.
+
+  Definition to_SemiRing_of_Monoid := SemiRing_of_Monoid.Axioms A
+    _ (mul f) (mulrA f) (mul1r f) (mulr1 f)
+    (mulrDl f) (mulrDr f) (mul0r) (mulr0).
+  Elpi hb.canonical A to_SemiRing_of_Monoid.
+
+Elpi hb.end.
+Elpi hb.structure Ring AbelianGroup.axioms Ring_of_AbelianGroup.axioms.
+
+Elpi hb.declare_factory Ring_of_Monoid A Monoid.axioms.
+  Record axioms := {
+    one : A;
+    opp : A -> A;
+    mul : A -> A -> A;
+    addNr : left_inverse zero opp add;
+    addrN : right_inverse zero opp add;
+    mulrA : associative mul;
+    mul1r : left_id one mul;
+    mulr1 : right_id one mul;
+    mulrDl : left_distributive mul add;
+    mulrDr : right_distributive mul add;
+  }.
+
+  Variable f : axioms.
+
+  Lemma addrC : commutative (add : A -> A -> A).
+  Proof.
+  have addKl (a b c : A) : a + b = a + c -> b = c.
+    apply: can_inj (add a) (add (opp f a)) _ _ _.
+    by move=> x; rewrite addrA (addNr f) add0r.
+  have addKr (a b c : A) : b + a = c + a -> b = c.
+    apply: can_inj (add ^~ a) (add ^~ (opp f a)) _ _ _.
+    by move=> x; rewrite /= -addrA (addrN f) addr0.
+  have innerC (a b : A) : a + b + (a + b) = a + a + (b + b).
+    by rewrite -[a+b](mul1r f) -(mulrDl f) (mulrDr f) !(mulrDl f) !(mul1r f).
+  move=> x y; apply: addKl (x) _ _ _; apply: addKr (y) _ _ _.
+  by rewrite -!addrA [in RHS]addrA innerC !addrA.
+  Qed.
+
+  Definition to_AbelianGroup_of_Monoid :=
+    AbelianGroup_of_Monoid.Axioms A (opp f) addrC (addNr f).
+  Elpi hb.canonical A to_AbelianGroup_of_Monoid.
+
+  Definition to_Ring_of_AbelianGroup :=
+    Ring_of_AbelianGroup.Axioms A (one f) (mul f)
+      (mulrA f) (mul1r f) (mulr1 f) (mulrDl f) (mulrDr f).
+  Elpi hb.canonical A to_Ring_of_AbelianGroup.
+
+Elpi hb.end.
+
+End V4.
 
 Import V3. (* or V1, both work! *)
 
